src/base/wpr_lifting.v
@@ -114,7 +114,7 @@ Section wpr.
     rewrite /valid_heap /valid_heap_lub.
     intros cut val.
     intros ℓ h look'.
-    rewrite /slice_of_store in look'.
+    rewrite /slice_of_store /slice_of_hist map_fmap_zip_with in look'.
     apply map_lookup_zip_with_Some in look'.
     destruct look' as ([t] & hist & ? & pLook & ?).
     eapply map_Forall_lookup_1 in val; last done.
@@ -128,7 +128,9 @@ Section wpr.
       rewrite eq.
       naive_solver.
     - rewrite H0.
-      destruct (hist !! t); simpl; last apply map_Forall_empty.
+      destruct (hist !! t);
+        [rewrite map_fmap_singleton|rewrite fmap_empty];
+        simpl; last apply map_Forall_empty.
       simplify_eq.
       apply map_Forall_singleton.
       apply view_empty_least.
@@ -202,7 +204,7 @@ Section wpr.
       * iRight. iPureIntro.
         eapply consistent_cut_lookup_slice; done.
       * iLeft.
-        rewrite /slice_of_store in look'.
+        rewrite /slice_of_store /slice_of_hist map_fmap_zip_with in look'.
         apply map_lookup_zip_with_Some in look'.
         destruct look' as ([t] & ? & ? & p'Look & ?).
         rewrite /consistent_cut in cut.
@@ -211,6 +213,7 @@ Section wpr.
         iExists _, _.
         iSplit; first done.
         rewrite H2.
+        rewrite map_fmap_singleton.
         iFrame "pts".
         iPureGoal; first done.
         iPureIntro.
@@ -221,8 +224,9 @@ Section wpr.
     * simpl.
       iSplit. { iPureIntro. apply store_inv_cut; done. }
       iExists p'. iFrame "crashed".
+      (* TODO: Factor this out into a lemma (needs [cut] only). *)
       apply consistent_cut_subseteq_dom in cut.
-      rewrite /slice_of_store.
+      rewrite /slice_of_store /slice_of_hist map_fmap_zip_with.
       rewrite map_zip_with_dom_eq_l; try done.
     * iModIntro.
       iIntros (V) "pers".
